LambdaS5/caml/desugar.mli
@@ -1,9 +1,9 @@
 
-val get_js_parser : unit -> (string -> Syntax.expr) option
+val get_js_parser : unit -> (string -> LjsSyntax.expr) option
 
 val set_js_parser_s5 : string -> unit
 
-val desugar_file : string -> Syntax.expr
+val desugar_file : string -> LjsSyntax.expr
 
-val desugar : string -> Syntax.expr
+val desugar : string -> LjsSyntax.expr
 
