LambdaS5/caml/eval.ml
@@ -1,7 +1,7 @@
 
 open Batteries
 
-open Syntax
+open LjsSyntax
 
 let usage_msg = "Usage: "
 
@@ -33,8 +33,8 @@ let save_store filename =
     File.with_file_out filename (fun ch -> Marshal.to_channel ch (get_store ()) [Marshal.Closures])
 
 let mk_env_vars () =
-    let props = List.map (function (s, _) -> (s, Syntax.Coq_property_data (Syntax.Coq_data_intro (Syntax.Coq_expr_id s, Syntax.Coq_expr_true, Syntax.Coq_expr_false, Syntax.Coq_expr_false)))) (HeapUtils.Heap.to_list (loc_heap (fst (get_store ())))) in
-    match Run.eval_ast (get_store ()) (Syntax.Coq_expr_seq (Syntax.Coq_expr_set_bang (String.to_list "%makeGlobalEnv", Syntax.Coq_expr_lambda ([], Syntax.Coq_expr_object (Translate.translate_attrs Ljs_syntax.d_attrs, props))), Syntax.Coq_expr_dump)) with
+    let props = List.map (function (s, _) -> (s, Coq_property_data (Coq_data_intro (Coq_expr_id s, Coq_expr_true, Coq_expr_false, Coq_expr_false)))) (HeapUtils.Heap.to_list (loc_heap (fst (get_store ())))) in
+    match Run.eval_ast (get_store ()) (Coq_expr_seq (Coq_expr_set_bang (String.to_list "%makeGlobalEnv", Coq_expr_lambda ([], Coq_expr_object (Translate.translate_attrs Ljs_syntax.d_attrs, props))), Coq_expr_dump)) with
         | Coq_result_dump (c, st) -> 
             store := Some (c, st)
         | r -> failwith "Internal error"
